Stlc/open_close.lean
@@ -8,13 +8,13 @@ Variable closing turns some free variables into bound variables.
 It is used to build an abstraction given a representation of its body. -/
 
 @[simp]
-def opening (x : ℕ) (a : Trm) : Trm → Trm
-| bvar i => if x = i then a else (bvar i)
-| fvar i => fvar i
-| abs u => abs (opening (x + 1) a u)
-| app u1 u2 => app (opening x a u1) (opening x a u2)
+def opening (k : ℕ) (u : Trm) : Trm → Trm
+| bvar i => if k = i then u else (bvar i)
+| fvar x => fvar x
+| abs t => abs (opening (k + 1) u t)
+| app t1 t2 => app (opening k u t1) (opening k u t2)
 
-notation " {" x " ~> " a "} " u => opening x a u
+notation " {" k " ~> " u "} " t => opening k u t
 
 -- Example of opening --
 #eval {0 ~> $2} λ(€0) --does not change since λ.0 is a closed term
@@ -24,50 +24,50 @@ notation " {" x " ~> " a "} " u => opening x a u
 
 
 --Opening at index zero
-def open₀ u a := opening 0 a u
+def open₀ t u := opening 0 u t
 
 lemma open_var_fv (t u: Trm) :
-    (j : ℕ) → fv (opening j u t) ⊆ (fv t) ∪ (fv u) := by
+    (k : ℕ) → fv (opening k u t) ⊆ (fv t) ∪ (fv u) := by
   induction t
   case bvar i =>
-    intro j
+    intro k
     simp [opening]
-    by_cases h : j = i
+    by_cases h : k = i
     . rw [if_pos h, fv]
       simp
     . rw [if_neg h, fv]
       simp
-  case fvar i =>
+  case fvar x =>
     simp [opening, fv]
-  case abs s hs =>
+  case abs t ht =>
     simp [opening, fv]
-    exact (fun j => hs (j + 1))
-  case app s1 s2 hs1 hs2 =>
+    exact (fun k => ht (k + 1))
+  case app t1 t2 ht1 ht2 =>
     simp [opening, fv]
-    intro j
-    apply (@Finset.Subset.trans ℕ _ ((fv s1 ∪ fv u) ∪ (fv s2 ∪ fv u)) _)
-    exact Finset.union_subset_union (hs1 j) (hs2 j)
+    intro k
+    apply (@Finset.Subset.trans ℕ _ ((fv t1 ∪ fv u) ∪ (fv t2 ∪ fv u)) _)
+    exact Finset.union_subset_union (ht1 k) (ht2 k)
     simp [Finset.union_assoc]
     refine Finset.union_subset_union_right ?_
     rw [Finset.union_comm]
     simp
 
-lemma opening_lc_lemma (e a b : Trm) :
+lemma opening_lc_lemma (t u v : Trm) :
     (i j: ℕ) → i ≠ j
-    → ({j ~> a} e) = ({i ~> b} ({j ~> a} e))
-    → e = ({i ~> b} e) := by
-  induction e
-  case bvar y =>
+    → ({j ~> u} t) = ({i ~> v} ({j ~> u} t))
+    → t = ({i ~> v} t) := by
+  induction t
+  case bvar k =>
    intro i j neqij h
-   by_cases hiy : (i = y)
-   . simp [opening, ← hiy] at h
-     rw [hiy]
+   by_cases hik : (i = k)
+   . simp [opening, ← hik] at h
+     rw [hik]
      rw [if_neg] at h
-     rwa [hiy] at h
+     rwa [hik] at h
      exact (fun hij => neqij (symm hij))
    . simp [opening]
      rw [if_neg]
-     exact hiy
+     exact hik
   case fvar y =>
    intro i j _ _
    rfl
@@ -89,10 +89,10 @@ lemma opening_lc_lemma (e a b : Trm) :
 def closing (k x : ℕ) : Trm → Trm
 | bvar i => bvar i
 | fvar i => if x = i then (bvar k) else (fvar i)
-| abs u => abs (closing (k + 1) x u)
-| app u1 u2 => app (closing k x u1) (closing k x u2)
+| abs t => abs (closing (k + 1) x t)
+| app t1 t2 => app (closing k x t1) (closing k x t2)
 
-notation " { " k " <~ " x " } " u => closing k x u
+notation " { " k " <~ " x " } " t => closing k x t
 
 -- Example of closing --
 #eval {0 <~ 2} λ($1) -- does not change since λx.1 does not contain the variable we want to change
@@ -100,38 +100,38 @@ notation " { " k " <~ " x " } " u => closing k x u
 #eval {0 <~ 4} λ(λ($4)) -- becomes λ(λ(€2)), it builds the abstraction λ.λ.λ.2 as expected
 
 --Closing at index zero
-def close₀ u a := closing 0 a u
+def close₀ u x := closing 0 x u
 
 lemma close_var_fv (t : Trm) (x : ℕ) :
-    (j : ℕ) → fv (closing j x t) = (fv t) \ {x} := by
+    (k : ℕ) → fv (closing k x t) = (fv t) \ {x} := by
   induction t
   case bvar _ =>
     simp [closing, fv]
-  case fvar i =>
-    intro j
+  case fvar y =>
+    intro k
     simp [closing, fv]
-    by_cases hi : x = i
-    . rw [if_pos hi, fv, hi]
+    by_cases hy : x = y
+    . rw [if_pos hy, fv, hy]
       simp
-    . rw [if_neg hi, fv]
-      simp [hi]
+    . rw [if_neg hy, fv]
+      simp [hy]
   case abs u hu =>
-    intro j
+    intro k
     simp [closing, fv]
-    exact (hu (j + 1))
+    exact (hu (k + 1))
   case app u1 u2 hu1 hu2 =>
-    intro j
+    intro k
     simp [closing, fv]
-    simp [hu1 j, hu2 j]
+    simp [hu1 k, hu2 k]
     exact Eq.symm (Finset.union_sdiff_distrib (fv u1) (fv u2) {x})
 
 ----------------------------------------------------------------------
 --Locally closed terms
 inductive lc : Trm → Prop
 | lc_var : ∀ x : ℕ, lc (fvar x)
-| lc_abs : ∀ a : Trm, ∀ L : Finset ℕ,
-   (∀ x : ℕ, x ∉ L → lc (open₀ a ($ x))) → lc (abs a)
-| lc_app : ∀ u1 u2 : Trm, lc u1 → lc u2 → lc (app u1 u2)
+| lc_abs : ∀ t : Trm, ∀ L : Finset ℕ,
+   (∀ x : ℕ, x ∉ L → lc (open₀ t ($ x))) → lc (abs t)
+| lc_app : ∀ t1 t2 : Trm, lc t1 → lc t2 → lc (app t1 t2)
 
 open lc
 
@@ -172,7 +172,7 @@ lemma lc_abs_iff_body : ∀ t, lc (abs t) ↔ body t := by
 are inverses of each other on variables.-/
 --1) Close(Open)=Id
 lemma close_open (x : ℕ) (t : Trm) :
-    x ∉ fv t → (j : ℕ) → closing j x (opening j ($ x) t) = t := by
+    x ∉ fv t → (k : ℕ) → closing k x (opening k ($ x) t) = t := by
   intro hx
   induction t
   case bvar i =>
@@ -185,7 +185,7 @@ lemma close_open (x : ℕ) (t : Trm) :
     . rw [if_neg]
       simp only [closing]
       exact hi
-  case fvar i =>
+  case fvar y =>
     simp [opening, closing]
     simp [fv] at hx
     exact hx
@@ -218,26 +218,26 @@ lemma open_close_lemma (x y z : ℕ) (t : Trm) : x ≠ y → y ∉ fv t
       = ({j ~> ($ z)} ({j <~ x} ({i ~> ($ y)} t))) ):= by
   intro neqxy hy
   induction t
-  case bvar a =>
+  case bvar k =>
     intro i j neqij
     simp only [opening]
-    by_cases hia : i = a
+    by_cases hik : i = k
     . simp only [closing, opening]
-      rw [if_pos hia]
+      rw [if_pos hik]
       rw [if_neg]
       simp only [opening, closing]
-      rw [if_pos hia, if_neg neqxy, opening]
-      exact (fun p => neqij (by rw [← p] at hia; exact hia))
-    . rw [if_neg hia]
+      rw [if_pos hik, if_neg neqxy, opening]
+      exact (fun p => neqij (by rw [← p] at hik; exact hik))
+    . rw [if_neg hik]
       simp [opening]
-      by_cases hja : j = a
-      . rw [if_pos hja]
+      by_cases hjk : j = k
+      . rw [if_pos hjk]
         simp only [opening]
-      . rw [if_neg hja]
+      . rw [if_neg hjk]
         simp only [opening, ite_eq_right_iff]
-        intro ia
+        intro ik
         simp
-        exact (hia ia)
+        exact (hik ik)
   case fvar a =>
     intro i j _
     simp only [closing]
@@ -262,7 +262,7 @@ lemma open_close_lemma (x y z : ℕ) (t : Trm) : x ≠ y → y ∉ fv t
     exact ⟨hu1 hy.1 i j neqij, hu2 hy.2 i j neqij⟩
 
 lemma open_close (x : ℕ) (t : Trm) :
-    lc t → (j : ℕ) → opening j ($ x) (closing j x t) = t := by
+    lc t → (k : ℕ) → opening k ($ x) (closing k x t) = t := by
   intro lct
   induction lct
   case lc_var y =>
@@ -310,102 +310,102 @@ lemma closing_injective (x i : ℕ) (t1 t2 : Trm) :
 
 -----------------------------------------
 --Auxilary lemma about opening
-lemma opening_lc (e a : Trm) : lc e → (i : ℕ) → (e = {i ~> a} e) := by
+lemma opening_lc (t u : Trm) : lc t → (k : ℕ) → (t = {k ~> u} t) := by
   intro lce
   induction lce
   case lc_var x =>
     intro _
     rfl
-  case lc_abs u L _ hu =>
+  case lc_abs v L _ hv =>
     intro i
-    simp [open₀] at hu
+    simp [open₀] at hv
     rw [opening]
     have  ⟨x, hx⟩ : ∃ x : ℕ, x ∉ L := by
       exact Infinite.exists_not_mem_finset L
-    have t : u = { i + 1 ~> a } u := by
-      apply (opening_lc_lemma u ($ x) a (i + 1) 0)
+    have h : v = { i + 1 ~> u } v := by
+      apply (opening_lc_lemma v ($ x) u (i + 1) 0)
       exact Nat.succ_ne_zero i
-      exact (hu x hx (i + 1))
-    rw [← t]
+      exact (hv x hx (i + 1))
+    rw [← h]
   case lc_app u1 u2 _ _ hu1 hu2 =>
     intro i
     simp [opening]
     exact ⟨hu1 i, hu2 i⟩
 
-lemma open₀_lc (e a : Trm) : lc e → (e = open₀ e a) := by
+lemma open₀_lc (t u : Trm) : lc t → (t = open₀ t u) := by
   intro lce
   simp [open₀]
-  apply (opening_lc e a lce 0)
+  apply (opening_lc t u lce 0)
 
 --Free variable substitution distributes over index substitution.
-lemma subst_open_rec (e1 e2 a : Trm) : (i j : ℕ) → lc a
-    → ([i // a] ({j ~> e2} e1)) = ({j ~> [i // a] e2} ([i // a] e1)) := by
-  induction e1
-  case bvar y =>
+lemma subst_open_rec (t1 t2 u : Trm) : (i j : ℕ) → lc u
+    → ([i // u] ({j ~> t2} t1)) = ({j ~> [i // u] t2} ([i // u] t1)) := by
+  induction t1
+  case bvar k =>
    intro i j _
-   by_cases hjy : (j = y)
+   by_cases hjk : (j = k)
    . simp [opening]
-     rw [if_pos, if_pos] <;> exact hjy
+     rw [if_pos, if_pos] <;> exact hjk
    . simp [opening]
      rw [if_neg, if_neg, subst]
-     <;> exact hjy
+     <;> exact hjk
   case fvar y =>
-   intro i j lca
+   intro i j lcu
    by_cases hyi : (y = i)
    . simp [opening, subst]
      rw [if_pos]
-     exact (opening_lc a ([ i // a ] e2) lca j)
+     exact (opening_lc u ([ i // u ] t2) lcu j)
      exact hyi
    . simp [opening, subst]
      rw [if_neg]
-     exact (opening_lc ($ y) ([ i // a ] e2) (lc.lc_var y) j)
+     exact (opening_lc ($ y) ([ i // u ] t2) (lc.lc_var y) j)
      exact hyi
-  case abs u hu =>
-   intro i j lca
+  case abs v hv =>
+   intro i j lcu
    simp [opening, subst]
-   exact (hu i (j + 1) lca)
+   exact (hv i (j + 1) lcu)
   case app u1 u2 hu1 hu2 =>
-   intro i j lca
+   intro i j lcu
    simp [opening, subst]
-   exact ⟨hu1 i j lca, hu2 i j lca ⟩
+   exact ⟨hu1 i j lcu, hu2 i j lcu⟩
 
 --The lemma above is most often used with k = 0 and e2 as some fresh variable.
 --Therefore, it simplifies matters to define the following useful corollary.
-lemma subst_open_var (e a : Trm) : lc a → (i j : ℕ) → i ≠ j
-    → (open₀ ([i // a] e) ($ j)) = ([i // a] (open₀ e ($ j))) := by
-  intro lca i j neqij
+lemma subst_open_var (t u : Trm) : lc u → (i j : ℕ) → i ≠ j
+    → (open₀ ([i // u] t) ($ j)) = ([i // u] (open₀ t ($ j))) := by
+  intro lcu i j neqij
   simp [open₀]
-  rw [subst_open_rec e ($ j) a i 0 lca]
+  rw [subst_open_rec t ($ j) u i 0 lcu]
   rw [subst, if_neg]
   exact (fun p => neqij (Eq.symm p))
 
 
 --When we open a term, we can instead open the term with a fresh variable and
 --then substitute for that variable.
-lemma subst_intro (e a : Trm) : lc a → (i : ℕ) → i ∉ (fv e)
-    → (open₀ e a) = ([i // a] (open₀ e ($ i))) := by
-  intro lca i hi
+lemma subst_intro (t u : Trm) : lc u → (x : ℕ) → x ∉ (fv t)
+    → (open₀ t u) = ([x // u] (open₀ t ($ x))) := by
+  intro lcu x hx
   simp [open₀]
-  rw [subst_open_rec e ($ i) a i 0 lca]
+  rw [subst_open_rec t ($ x) u x 0 lcu]
   rw [subst, if_pos]
   rw [subst_fresh]
-  exact hi
+  exact hx
   rfl
 
-lemma subst_lc (e a : Trm) : (x : ℕ) → lc e → lc a → lc ([x // a] e) := by
-  intro x lce lca
-  induction lce
+lemma subst_lc (t u : Trm) : (x : ℕ) → lc t → lc u → lc ([x // u] t) := by
+  intro x lct lcu
+  induction lct
   case lc_var y =>
     rw [subst]
     by_cases hxy : y = x
     . rw [if_pos]
-      exact lca
+      exact lcu
       exact hxy
     . rw [if_neg]
       exact (lc_var y)
       exact hxy
-  case lc_abs u L _ hu =>
-    apply (lc_abs ([ x // a ] u) (L ∪ {x}))
+  case lc_abs v L _ hv =>
+    apply (lc_abs ([ x // u ] v) (L ∪ {x}))
     intro x₀ hx₀
     have t1 : x₀ ∉ L := by
       intro s
@@ -414,11 +414,11 @@ lemma subst_lc (e a : Trm) : (x : ℕ) → lc e → lc a → lc ([x // a] e) := 
       simp at hx₀
       push_neg at hx₀
       exact hx₀.2
-    rw [subst_open_var u a lca x x₀ t2.symm]
-    exact (hu x₀ t1)
-  case lc_app u1 u2 lcu1 lcu2 hu1 hu2 =>
+    rw [subst_open_var v u lcu x x₀ t2.symm]
+    exact (hv x₀ t1)
+  case lc_app t1 t2 lct1 lct2 ht1 ht2 =>
     dsimp [subst]
-    apply (lc_app ( [ x // a ] u1) ( [ x // a ] u2) hu1 hu2)
+    apply (lc_app ( [ x // u ] t1) ( [ x // u ] t2) ht1 ht2)
 
 lemma open_var_body : ∀ x t, body t → lc (open₀ t ($ x)) := by
   intro x t bt
@@ -453,23 +453,23 @@ lemma open_lc : ∀ t u, lc (abs t) → lc u → lc (open₀ t u) := by
   exact (open_body t u lcat lcu)
 
 lemma open_close_subst t x y :
-    lc t → (∀ z, (opening z ($ y) (closing z x t)) = ([x // ($ y)] t)) := by
+    lc t → (∀ k, (opening k ($ y) (closing k x t)) = ([x // ($ y)] t)) := by
   intro lct
   induction lct
-  case lc_var k =>
+  case lc_var y =>
     simp only [closing, subst]
-    by_cases hxk : x = k
-    . simp [if_pos hxk, if_pos hxk.symm]
-    . have hkx : k ≠ x := (fun p => (hxk p.symm))
-      simp [if_neg hxk, if_neg hkx]
+    by_cases hxy : x = y
+    . simp [if_pos hxy, if_pos hxy.symm]
+    . have hyx : y ≠ x := (fun p => (hxy p.symm))
+      simp [if_neg hxy, if_neg hyx]
   case lc_abs s L f h =>
     simp [opening, subst, abs.injEq]
-    intro z
-    let ⟨w, qw⟩ := pick_fresh s (L ∪ {x} ∪ (fv ( {z + 1 ~> $ y} { z + 1 <~ x } s)) ∪ (fv ([x // $ y] s)))
+    intro k
+    let ⟨w, qw⟩ := pick_fresh s (L ∪ {x} ∪ (fv ( {k + 1 ~> $ y} { k + 1 <~ x } s)) ∪ (fv ([x // $ y] s)))
     simp at qw
     push_neg at qw
     have hwx : x ≠ w := (fun p => (qw.2.1 p.symm))
-    have fact := h w qw.1 (z + 1)
+    have fact := h w qw.1 (k + 1)
     rw [← subst_open_var _ _ (lc_var y) _ _ hwx, open₀] at fact
     rw [← open_close_lemma _ _ _ _ hwx, ← open₀] at fact
     apply open₀_injective w _
@@ -479,6 +479,6 @@ lemma open_close_subst t x y :
     exact qw.2.2.2.2
     exact Nat.ne_of_beq_eq_false rfl
   case lc_app u1 u2 _ _ f1 f2 =>
-    intro z
+    intro k
     simp
-    exact ⟨f1 z, f2 z⟩
+    exact ⟨f1 k, f2 k⟩
